cas/theories/App.v
@@ -38,7 +38,7 @@ Definition clientT := nat.
 
 Variant appE {exp_} : Type -> Type :=
   App__Send : clientT -> responseT exp_ -> appE unit
-| App__Recv : server_state exp_ -> appE (clientT * requestT).
+| App__Recv : server_state exp_ -> appE (clientT * requestT id).
 Arguments appE : clear implicits.
 
 Variant symE {exp_} : Type -> Type :=
@@ -74,18 +74,18 @@ Definition cas_smi {E R} `{Is__smE E} : itree E R :=
        match req with
        | Request__GET k t =>
          let get_handler tx vx st1 :=
-             ifx (Exp__Match t tx)
+             ifx (Exp__Match (t : id tag) tx)
                  (embed App__Send c Response__NotModified)
                  (embed App__Send c (Response__OK tx vx));;
              ret st1 in
          handle k get_handler
        | Request__CAS k t v =>
          let cas_handler tx _ st1 :=
-             ifx (Exp__Match t tx)
+             ifx (Exp__Match (t : id tag) tx)
                  (embed App__Send c Response__NoContent;;
                   tx1 <- trigger Sym__Fresh;;
                   ret (update k (tx1, Exp__Const v) st1))
                  (embed App__Send c Response__PreconditionFailed;;
-                  ret st1) in
+                  ret st1)in
          handle k cas_handler
        end) [].
